A more complex inductive proposition about hashing to be used by the checksummed log

src/Hashmap.v
@@ -12,6 +12,12 @@ Set Implicit Arguments.
 Definition hash2 sz1 sz2 (a : word sz1) (b : word sz2) :=
   hash_fwd (Word.combine a b).
 
+(** hash_list_rep takes in a list of values vl, a hash h, and a hashmap hm.
+    h is the hash of the values in vl:
+      h = hash( vl[n-1] || ... hash(vl[0] || default_hash))
+    When the list of values is empty, h must be equal to the default hash
+    value.
+*)
 Inductive hash_list_rep : (list valu) -> word hashlen -> hashmap -> Prop :=
   | HL_nil : forall hl hm,
       hl = hash_fwd default_valu ->
@@ -22,6 +28,24 @@ Inductive hash_list_rep : (list valu) -> word hashlen -> hashmap -> Prop :=
       hashmap_get hm hl' = Some (existT _ _ (Word.combine x hl)) ->
       hash_list_rep (x :: l) hl' hm.
 
+(** hash_list_prefixes takes in a list of values vl, a list of hashes hl,
+    and a hashmap hm. For each index i in hl, hl[i] must be equal to the
+    hash of the list vl[:i+1].
+    TODO: This could probably be merged into hash_list_rep, but not sure
+    how much more work that would be right now.
+*)
+Inductive hash_list_prefixes : list valu -> list (word hashlen) -> hashmap -> Prop :=
+  | HLP_default : forall hm,
+    hash_list_prefixes nil nil hm
+  | HLP_cons : forall v h vl hl hm,
+    hash_list_rep (v :: vl) h hm ->
+    hash_list_prefixes vl hl hm ->
+    hash_list_prefixes (v :: vl) (h :: hl) hm.
+
+(** hashmap_subset takes in a list hkl of (hash, key) pairs and two
+    hashmaps hm and hm'. hm' is equal to hm updated with all of the
+    pairs in hkl.
+*)
 Inductive hashmap_subset : list (word hashlen * {sz : nat & word sz}) -> hashmap -> hashmap -> Prop  :=
   | HS_nil : forall hm,
       hashmap_subset nil hm hm
@@ -34,8 +58,10 @@ Inductive hashmap_subset : list (word hashlen * {sz : nat & word sz}) -> hashmap
 Ltac existT_wordsz_neq H :=
   let Hx := fresh in
   inversion H as [ Hx ];
-  rewrite <- plus_0_r in Hx at 1;
-  apply plus_reg_l in Hx;
+  try (rewrite <- plus_0_r in Hx at 1;
+      apply plus_reg_l in Hx);
+  try (rewrite <- plus_0_r in Hx;
+      apply plus_reg_l in Hx);
   inversion Hx.
 
 Ltac existT_wordsz_eq H :=
@@ -51,6 +77,19 @@ Ltac contradict_hashmap_get_default H hm :=
   destruct (weq (hash_fwd default_valu) (hash_fwd default_valu));
   intro Hx; try existT_wordsz_neq Hx;
   intuition.
+
+Lemma hashmap_hashes_neq : forall hm h1 h2 sz1 sz2 (k1 : word sz1) (k2 : word sz2),
+  hashmap_get hm h2 = Some (existT _ _ k2) ->
+  hash_safe hm h1 k1 ->
+  Some (existT _ _ k1) <> Some (existT _ _ k2) ->
+  h1 <> h2.
+Proof.
+  unfold hash_safe.
+  intuition; subst;
+  rewrite H3 in H; inversion H.
+  existT_wordsz_eq H4.
+  intuition.
+Qed.
 
 Theorem hashmap_get_default : forall hm,
   hashmap_get hm default_hash = Some (existT _ _ default_valu).
@@ -94,6 +133,39 @@ Proof.
   inversion H. subst.
   apply hash_list_rep_upd; auto.
   eapply IHhkl; eauto.
+Qed.
+
+Theorem hash_list_injective : forall l1 l2 hv hm,
+  hash_list_rep l1 hv hm -> hash_list_rep l2 hv hm -> l1 = l2.
+Proof.
+  induction l1;
+    intros;
+    inversion H; inversion H0;
+    unfold hash2 in *; intuition;
+    subst; auto.
+
+  contradict_hashmap_get_default H6 hm.
+
+  rewrite H8 in H7.
+  contradict_hashmap_get_default H7 hm.
+
+  rewrite H7 in H10.
+  inversion H10.
+  existT_wordsz_eq H2.
+  intuition.
+  apply IHl1 in H8; congruence.
+Qed.
+
+Theorem hash_list_injective2 : forall l h1 h2 hm,
+  hash_list_rep l h1 hm -> hash_list_rep l h2 hm -> h1 = h2.
+Proof.
+  induction l; intros.
+  inversion H; inversion H0; subst. auto.
+
+  inversion H; inversion H0; subst.
+  assert (Heq: hl = hl0).
+    eapply IHl; eauto.
+  subst. auto.
 Qed.
 
 Theorem hash_safe_eq : forall hm h1 h2 sz (k1 k2 : word sz),
@@ -160,6 +232,92 @@ Proof.
 
   rewrite <- app_comm_cons.
   constructor; eauto.
+Qed.
+
+Theorem hashmap_get_subset : forall hm2 hm1 h k l,
+  hashmap_get hm1 h = Some k ->
+  hashmap_subset l hm1 hm2 ->
+  hashmap_get hm2 h = Some k.
+Proof.
+  induction hm2; intros.
+  inversion H0; subst; auto.
+
+  inversion H0; subst; auto.
+  destruct (weq h default_hash).
+  rewrite e in *.
+  rewrite hashmap_get_default in *; auto.
+
+  destruct (weq w h); subst.
+  rewrite upd_hashmap_eq; auto.
+  unfold hash_safe in *.
+  eapply IHhm2 in H; eauto.
+  rewrite H in *. intuition. inversion H1.
+
+  simpl.
+  destruct (weq h default_hash); intuition.
+  destruct (weq w h); intuition.
+  eapply IHhm2; eauto.
+Qed.
+
+(*Lemma hash_list_prefixes_forall : forall i vl hl hm default defaultv,
+  hash_list_prefixes vl hl hm ->
+  i < length hl - 1 ->
+  selN hl i default = hash2 (selN vl i defaultv) (selN hl (i + 1) default).
+Proof.
+  induction i; intros.
+  destruct hl. inversion H0.
+  destruct vl. inversion H.
+
+  inversion H; subst.
+  simpl. inversion H7.
+  rewrite <- H2 in H0. inversion H0.
+  simpl.
+  inversion H6; subst.
+  eapply hash_list_injective2 in H1; eauto.
+  subst; auto.
+
+  destruct hl. inversion H0.
+  destruct vl. inversion H.
+
+  simpl.
+  eapply IHi.
+  inversion H; subst. eauto.
+  simpl in *. omega.
+Qed.*)
+
+
+Theorem hash_list_prefixes_upd : forall vl hl hm h sz (k : word sz),
+  hash_list_prefixes vl hl hm ->
+  hash_safe hm h k ->
+  hash_list_prefixes vl hl (upd_hashmap' hm h k).
+Proof.
+  induction vl; intros.
+  inversion H; subst. constructor.
+
+  inversion H; subst.
+  constructor.
+  apply hash_list_rep_upd; auto.
+  eapply IHvl; auto.
+Qed.
+
+Theorem hash_list_prefixes_subset : forall l hm1 hm2 vl hl,
+  hashmap_subset l hm1 hm2 ->
+  hash_list_prefixes vl hl hm1 ->
+  hash_list_prefixes vl hl hm2.
+Proof.
+  induction l; intros.
+  inversion H; subst; auto.
+
+  inversion H; subst.
+  apply hash_list_prefixes_upd.
+  eapply IHl; eauto. auto.
+Qed.
+
+Lemma upd_hashmap_neq : forall hm h k,
+  hm <> upd_hashmap hm h k.
+Proof.
+  induction hm; intuition; inversion H; intuition.
+  eapply IHhm; eauto.
 Qed.
 
 (** Chains together hashmap_subset patterns until it solves the goal.
